Partial fix to Capacity() issues

Source/DafnyStandardLibraries/src/Std/Actions/Consumers.dfy
@@ -42,9 +42,48 @@ module Std.Consumers {
     }
   }
 
+  datatype ConsumerState<T> = ConsumerState(consumer: Consumer<T>, capacity: Option<nat>, history: seq<(T, bool)>){
+    ghost predicate Valid() {
+      && Seq.Partitioned(history, WasConsumed)
+      && (!Seq.All(history, WasConsumed) && capacity.Some? ==> capacity.value == 0)
+    }
+    ghost predicate ValidChange(newer: ConsumerState<T>) 
+    {
+      && newer.consumer == consumer
+      && Valid()
+      && newer.Valid()
+      && history <= newer.history
+      && var newHistory := newer.history[|history|..];
+        assert newer.history == history + newHistory;
+        Seq.PartitionedDecomposition(history, newHistory, WasConsumed);
+        ConsumedComposition(history, newHistory);
+      && var newConsumed := ConsumedOf(newHistory);
+      && capacity.Some? ==>
+        && |newConsumed| <= capacity.value
+        && (!Seq.All(newer.history, WasConsumed) ==> |newConsumed| == capacity.value)
+        && newer.capacity == Some(capacity.value - |newConsumed|)
+    }
+
+    ghost function NewConsumed(newer: ConsumerState<T>): seq<T>
+      requires ValidChange(newer)
+    {
+      var newHistory := newer.history[|history|..];
+      assert newer.history == history + newHistory;
+      Seq.PartitionedDecomposition(history, newHistory, WasConsumed);
+      ConsumedOf(newHistory)
+    }
+  }
+
   // Actions that attempt to consume a T and eventually reach capacity and fail.
   @AssumeCrossModuleTermination
   trait Consumer<T> extends Action<T, bool> {
+
+    ghost function State(): ConsumerState<T>
+      requires Valid()
+      reads this, Repr
+    {
+      ConsumerState(this, Capacity(), history)
+    }
 
     twostate predicate ValidChange()
       reads this, Repr
@@ -52,10 +91,10 @@ module Std.Consumers {
       ensures ValidChange() ==> fresh(Repr - old(Repr))
       ensures ValidChange() ==> old(history) <= history
     {
+      && old(Valid()) && Valid()
       && fresh(Repr - old(Repr))
-      && old(Valid())
-      && Valid()
       && old(history) <= history
+      && old(State()).ValidChange(State())
     }
 
     // Termination metric ensuring Accept() eventually returns false.
@@ -94,23 +133,29 @@ module Std.Consumers {
       !Seq.All(Outputs(), IsTrue)
     }
 
+    ghost predicate ValidHistory(history: seq<(T, bool)>)
+      decreases Repr
+    {
+      Seq.Partitioned(history, WasConsumed)
+    }
+
     function Capacity(): Option<nat>
       reads this, Repr
       requires Valid()
 
-    // ghost function Consumed(): seq<T> {
-    //   Seq.Count(IsTrue, Outputs())
-    // }
+    ghost function Consumed(): seq<T>
+      requires ValidHistory(history)
+      reads this, Repr
+    {
+      ConsumedOf(history)
+    }
 
-    // twostate function NewConsumed(): seq<T> {
-    //   Consumed() - old(Consumed())
-    // }
-
-    // twostate lemma CapacityCorrect()
-    //   requires ValidChange()
-    //   requires old(Capacity()).Some?
-    //   ensures |NewConsumed()| < old(Capacity()).value
-    //   ensures Done() ==> |NewConsumed()| == old(Capacity()).value
+    twostate function NewConsumed(): seq<T>
+      requires ValidChange()
+      reads this, Repr
+    {
+      old(State()).NewConsumed(State())
+    }
 
     method Invoke(t: T) returns (r: bool)
       requires Requires(t)
@@ -143,6 +188,69 @@ module Std.Consumers {
     b == false
   }
 
+  predicate WasConsumed<T>(pair: (T, bool)) {
+    pair.1
+  }
+
+  predicate WasNotConsumed<T>(pair: (T, bool)) {
+    !pair.1
+  }
+
+  ghost function ConsumedOf<T>(history: seq<(T, bool)>): seq<T>
+    requires Seq.Partitioned(history, WasConsumed)
+  {
+    if history == [] then
+      []
+    else
+      var (input, accepted) := history[0];
+      if accepted then
+        [input] + ConsumedOf(history[1..])
+      else
+        ConsumedOf(history[1..])
+  }
+
+  lemma ConsumedOfAllNotConsumedEmpty<T>(history: seq<(T, bool)>)
+    requires Seq.AllNot(history, WasConsumed)
+    ensures ConsumedOf(history) == []
+  {}
+
+  @IsolateAssertions
+  lemma ConsumedComposition<T>(left: seq<(T, bool)>, right: seq<(T, bool)>)
+    requires Seq.Partitioned(left, WasConsumed)
+    requires Seq.Partitioned(right, WasConsumed)
+    requires Seq.Partitioned(left + right, WasConsumed)
+    ensures ConsumedOf(left + right) == ConsumedOf(left) + ConsumedOf(right)
+  {
+    var combined := left + right;
+    if left == [] {
+      assert left + right == right;
+    } else {
+      if !left[0].1 {
+        assert !combined[0].1;
+        Seq.PartitionedFirstFalseImpliesAllNot(combined, WasConsumed);
+        Seq.AllNotDecomposition(left, right, WasConsumed);
+        ConsumedOfAllNotConsumedEmpty(left);
+        ConsumedOfAllNotConsumedEmpty(right);
+        ConsumedOfAllNotConsumedEmpty(left + right);
+        assert ConsumedOf(left) == ConsumedOf(right) == [];
+        assert ConsumedOf(left + right) == ConsumedOf(left) + ConsumedOf(right);
+      } else {
+        assert ConsumedOf(left) == [left[0].0] + ConsumedOf(left[1..]);
+        assert Seq.Partitioned(left[1..], WasConsumed);
+        assert left + right == [left[0]] + (left[1..] + right);
+        assert Seq.Partitioned([left[0]] + (left[1..] + right), WasConsumed);
+        Seq.PartitionedDecomposition([left[0]], left[1..] + right, WasConsumed);
+        assert Seq.Partitioned(left[1..] + right, WasConsumed);
+        assert ConsumedOf(left + right) == [left[0].0] + ConsumedOf(left[1..] + right);
+        assert Seq.Partitioned(left[1..] + right, WasConsumed);
+
+        ConsumedComposition(left[1..], right);
+
+        assert ConsumedOf(left + right) == ConsumedOf(left) + ConsumedOf(right);
+      }
+    }
+  }
+
   @AssumeCrossModuleTermination
   class ArrayWriter<T> extends Consumer<T> {
 
@@ -157,9 +265,12 @@ module Std.Consumers {
       decreases Repr, 0
     {
       && this in Repr
+      && ValidHistory(history)
       && storage in Repr
       && size <= storage.Length
-      && Inputs() == storage[..size]
+      && (Done() ==> size == storage.Length)
+      && Consumed() == storage[..size]
+      && (size < storage.Length ==> Seq.All(history, WasConsumed))
     }
 
     twostate lemma ValidImpliesValidChange()
@@ -167,7 +278,7 @@ module Std.Consumers {
       requires unchanged(old(Repr))
       ensures ValidChange()
     {}
-    
+
     constructor (storage: array<T>)
       ensures Valid()
       ensures history == []
@@ -176,13 +287,11 @@ module Std.Consumers {
       Repr := {this} + {storage};
       this.storage := storage;
       this.size := 0;
+      new;
+      assert ConsumedOf(history) == [];
+      assert storage[..size] == [];
     }
 
-    ghost predicate ValidHistory(history: seq<(T, bool)>)
-      decreases Repr
-    {
-      true
-    }
     ghost predicate ValidInput(history: seq<(T, bool)>, next: T)
       decreases Repr
     {
